Enc proof done

proof/X-Wing-Correction-Proof.ec
@@ -2,11 +2,9 @@ require import AllCore IntDiv CoreMap List Distr IntDiv StdOrder.
 
 from Jasmin require import JModel_x86 JModel JWord JUtils.
 
-
-
 import SLH64 StdOrder.IntOrder.
 require import Xkem_avx2_clean  XWing_Spec XWing_Helper_Functions CorrectnessProof_Mulx Mulx_scalarmult_s Jkem_avx2_stack FIPS202_SHA3 Curve25519_Procedures MLKEM MLKEM_KEM_avx2_stack Symmetric.
-require import Array4 Array6 Array8 Array32 Array64 Array96 Array140 Array152 Array1088 Array1120 Array1184 Array1216 Array2400 Array1152.
+require import Array4 Array6 Array8 Array32 Array64 Array96 Array140 Array152 Array128 Array960 Array1088 Array1120 Array1184 Array1216 Array2400 Array1152.
 require import WArray4 WArray6 WArray32 WArray64 WArray96 WArray1088 WArray1120 WArray1184 WArray1216 WArray2400.
 
 axiom shake256_A96_A32 out inp :
@@ -316,4 +314,226 @@ proof.
    wp. auto => />. rewrite !tP.
    move => &1 &2 H H0 H1 H2 H3 H4 H5 H6. move => i ib. rewrite initiE 1,2:/#.
    wp. auto => />.
+qed.
+
+
+lemma copy1216 (a : W8.t Array1216.t) :
+Array1216.init (fun (i : int)  =>  WArray1216.get8 (WArray1216.init64
+               (fun (i0 : int) =>  copy_64 (Array152.init
+               (fun (i1 : int) =>  WArray1216.get64 (WArray1216.init8
+               (fun (i2 : int) =>  a.[i2]))  i1)).[i0])) i) = a.
+rewrite tP => k kb.
+rewrite initiE 1:/# /= /get8.
+rewrite initiE 1:/# /= /copy_64.
+rewrite initiE 1:/# /= /get64_direct.
+rewrite W8u8.pack8bE 1:/# /=.
+rewrite initiE 1:/# /=.
+rewrite initiE /#.
+qed.
+
+
+lemma eq_spec_xwing_enc:
+  equiv [Xkem_avx2_clean.M._crypto_xkem_enc_derand_jazz ~ XWing.enc_derand :
+      coins{2}.`1 = Array32.init (fun (i:int) => eseed{1}.[i])
+   /\ coins{2}.`2 = Array32.init (fun (i:int) => eseed{1}.[i + 32])
+   /\ pk{2}.`1.`1 = Array1152.init(fun i => pkp{1}.[i])
+   /\ pk{2}.`1.`2 = Array32.init(fun i => pkp{1}.[i+1152])
+   /\ pk{2}.`2    = Array32.init(fun i => pkp{1}.[i+1184])
+      ==>
+      res{2}.`1.`1.`1 = Array960.init(fun i => res{1}.`1.[i])
+   /\ res{2}.`1.`1.`2 = Array128.init(fun i => res{1}.`1.[i+960])
+   /\ res{2}.`1.`2    = Array32.init(fun i => res{1}.`1.[i+1088])
+   /\ res{2}.`2 = res{1}.`2].
+proof.
+    proc => />.
+    proc rewrite {1} 12 (copy1216).
+    proc rewrite {1} 13 (copy64).
+
+    seq 13 0 : (#pre /\ spkp{1} = pkp{1} /\ spkp{1} = pkp{1} /\ seseed{1} = eseed{1}).
+    + auto => />.
+
+    seq 1 1  : (#pre /\ pk_M{2}.`1 = Array1152.init (fun (i:int) => pk_mlkem{1}.[i])
+                     /\ pk_M{2}.`2 = Array32.init (fun (i:int) => pk_mlkem{1}.[i+1152])
+                     /\ pk_M{2}.`1 = Array1152.init (fun (i:int) => pkp{1}.[i])
+                     /\ pk_M{2}.`2 = Array32.init (fun (i:int) => pkp{1}.[i+1152])).
+    + auto => />. rewrite !tP. move => &1 &2 [#] H H0 H1 H2 H3. do split.
+    + move => i ib. rewrite !initiE 1,2:/# H1 1:/#. rewrite !initiE 1,2:/#.
+    + move => i ib. rewrite !initiE 1:/# //= H2 1:/#. rewrite !initiE 1,2:/# //=.
+
+    seq 1 1  : (#pre /\ pk_X{2} = Array32.init (fun (i:int) => pk_x25519{1}.[i])
+                     /\ pk_X{2} = Array32.init (fun (i:int) => pkp{1}.[i+1184])).
+    + auto => />. rewrite !tP. move => &1 &2 [#] H H0 H1 H2 H3 H4 H5 H6 H7 H8 H9.
+    + rewrite !initiE 1,2:/# //= H3 1:/#. rewrite !initiE 1,2:/#.
+
+    seq 1 1  : (#pre /\ ek_X{2} = Array32.init (fun (i:int) => ek_x25519{1}.[i])
+                     /\ ek_X{2} = Array32.init (fun (i:int) => seseed{1}.[i+32])).
+    + auto => />. rewrite !tP. move => &1 &2 [#] H H0 H1 H2 H3 H4 H5 H6 H7 H8 H9 H10.
+    + rewrite !initiE 1,2:/# //= H0 1:/#. rewrite !initiE 1,2:/#.
+    swap{1} 3 -2.
+    seq 1 1  : (#pre /\ c_M{2} = seed_mlkem{1}
+                     /\ c_M{2} = Array32.init (fun (i:int) => seseed{1}.[i])).
+    + auto => />.
+    seq 1 1 : (#pre /\ pack32 (to_list ct_x25519{1}) = ct_X_256{2}).
+    + call eq_spec_xwing_25519_base_mulx. auto => />.
+    + move => &1 &2 H H0 H1 H2 H3 H4 H5 H6 H7 H8 H9.
+    + congr. congr. congr. rewrite tP => *. smt(Array32.initiE).
+
+    seq 1 1 : (#pre /\ pack32 (to_list ss_x25519{1}) = ss_X_256{2}).
+    + call eq_spec_xwing_25519_mulx. auto => />.
+    + move => &1 &2 H H0 H1 H2 H3 H4 H5 H6 H7 H8 H9. do split.
+    + congr. congr. congr. rewrite tP => *. smt(Array32.initiE).
+    + congr. congr. congr. rewrite tP => *. smt(Array32.initiE).
+
+    seq 0 1 : (#pre /\ ct_X{2} = ct_x25519{1}).
+    + auto => />. move => &1 &2 H H0 H1 H2 H3 H4 H5 H6 H7 H8 H9.
+    rewrite !/of_list !/to_list !/mkseq -iotaredE => />.
+    rewrite tP => i ib. rewrite initiE 1,2:/#.
+
+    seq 0 1 : (#pre /\ ss_X{2} = ss_x25519{1}).
+    + auto => />. move => &1 &2 H H0 H1 H2 H3 H4 H5 H6 H7 H8 H9.
+    rewrite !/of_list !/to_list !/mkseq -iotaredE => />.
+    rewrite tP => i ib. rewrite initiE 1,2:/#.
+
+   seq 2 3 : (#pre /\ ct_M{2}.`1 = Array960.init(fun i => ct_mlkem{1}.[i])
+                   /\ ct_M{2}.`2 = Array128.init(fun i => ct_mlkem{1}.[i+960])
+                   /\ ct{2}.`1.`1 = Array960.init(fun i => ct_mlkem{1}.[i])
+                   /\ ct{2}.`1.`2 = Array128.init(fun i => ct_mlkem{1}.[i+960])
+                   /\ ct{2}.`2 = Array32.init (fun i => ct_X{2}.[i])
+                   /\ ct{2}.`2 = ct_x25519{1}
+                   /\ ct_x25519{1} = ct_X{2}
+                   /\ ct_M{2}.`1 = ct{2}.`1.`1
+                   /\ ct_M{2}.`2 = ct{2}.`1.`2
+                   /\ ss_M{2} = ss_mlkem{1}
+                   /\ ={ss}).
+    + inline {2} 2. wp; sp.
+    + ecall {1} (sha3_256_A128__A6 ss{1} ss_mlkem{1} ss_x25519{1} ct_x25519{1} pk_x25519{1}).
+    + call mlkem_kem_correct_enc. auto => />.
+    + move => &1 &2 H H0 H1 H2 H3 H4 H5 H6 H7 H8 H9 H10 H11 H12.
+    + do split;1..4:smt(). rewrite tP => i ib. smt(Array32.initiE). smt().
+    + congr. congr. smt(). + rewrite tP => i ib. smt(Array32.initiE).
+
+    wp. auto => />.
+    auto => />.
+    + seq 3 0 : (#pre  /\ ct{2}.`1.`1 = Array960.init(fun i => ctp{1}.[i])
+                       /\ ct{2}.`1.`2 = Array128.init(fun i => ctp{1}.[i+960])
+                       /\ ct{2}.`1.`1 = Array960.init(fun i => ct_mlkem{1}.[i])
+                       /\ ct{2}.`1.`2 = Array128.init(fun i => ct_mlkem{1}.[i+960])
+                       /\ ct_M{2}.`1 = Array960.init(fun i => ctp{1}.[i])
+                       /\ ct_M{2}.`2 = Array128.init(fun i => ctp{1}.[i+960])
+                       /\ ct_M{2}.`1 = ct{2}.`1.`1
+                       /\ ct_M{2}.`2 = ct{2}.`1.`2
+                       /\ ct_X{2} = ct{2}.`2).
+
+    + while{1} (#pre /\ aux{1} = 136
+                     /\ ct{2}.`1.`1 = Array960.init(fun i => ct_mlkem{1}.[i])
+                     /\ ct{2}.`1.`2 = Array128.init(fun i => ct_mlkem{1}.[i+960])
+                     /\ ct_M{2}.`1 = Array960.init(fun i => ct_mlkem{1}.[i])
+                     /\ ct_M{2}.`2 = Array128.init(fun i => ct_mlkem{1}.[i+960])
+                     /\ ct_X{2} = ct_x25519{1}
+                     /\ (forall k, 0<=k<min (8 * i{1}) 960 => ctp{1}.[k] = ct_mlkem{1}.[k])
+                     /\ (forall k, 960<=k<min (8 * i{1}) 1088 => ctp{1}.[k] = ct_mlkem{1}.[k])
+                     /\ (forall k, 0<=k<min (8 * i{1}) 960 => ctp{1}.[k] = ct{2}.`1.`1.[k])
+                     /\ (forall k, 960<=k<min (8 * i{1}) 1088 => ctp{1}.[k] = ct{2}.`1.`2.[k-960])
+                     /\ (forall k, 0<=k<min (8 * i{1}) 960 => ctp{1}.[k] = ct_M{2}.`1.[k])
+                     /\ (forall k, 960<=k<min (8 * i{1}) 1088 => ctp{1}.[k] = ct_M{2}.`2.[k-960]))
+              (136 - i{1}).
+    + auto => />. move => &hr Z. rewrite !tP.
+    + move => H H0 H1 H2 H3 H4 H5 H6 H7 H8 H9 H10 H11 H12 H13 H14 H15 H16 H17 H18 H19 H20 *. do split.
+    + move => i b *. rewrite !initiE 1:/# get8_set64_directE 1,2:/#.
+    + case(8 * i{!hr} <= i && i < 8 * i{!hr} + 8) => *.
+    + rewrite get64E /init8 pack8bE 1:/# !initiE 1:/# //= !initiE 1:/# //= /#.
+    + rewrite /get8 /init8  -H16 1:/# !initiE 1:/# //=.
+    + move => i b *. rewrite !initiE 1:/# get8_set64_directE 1,2:/#.
+    + case(8 * i{!hr} <= i && i < 8 * i{!hr} + 8) => *.
+    + rewrite get64E /init8 pack8bE 1:/# !initiE 1:/# //= !initiE 1:/# //= /#.
+    + rewrite /get8 /init8. rewrite -H17 1:/# !initiE 1:/# //=.
+    + move => i b *. rewrite H11 1:/#.
+    + rewrite !initiE 1,2:/# get8_set64_directE 1,2:/#.
+    + case(8 * i{!hr} <= i && i < 8 * i{!hr} + 8) => *.
+    + rewrite get64E /init8 pack8bE 1:/# !initiE 1:/# //= !initiE 1:/# //= /#.
+    + rewrite /get8 /init8. rewrite -H16 1:/# !initiE 1:/# //=.
+    + move => i b *. rewrite H12 1:/#.
+    + rewrite !initiE 1,2:/# get8_set64_directE 1,2:/#.
+    + case(8 * i{!hr} <= i && i < 8 * i{!hr} + 8) => *.
+    + rewrite get64E /init8 pack8bE 1:/# !initiE 1:/# //= !initiE 1:/# //= /#.
+    + rewrite /get8 /init8. rewrite -H17 1:/# !initiE 1:/# //=.
+    + move => i b *. rewrite H9 1:/#.
+    + rewrite !initiE 1,2:/# get8_set64_directE 1,2:/#.
+    + case(8 * i{!hr} <= i && i < 8 * i{!hr} + 8) => *.
+    + rewrite get64E /init8 pack8bE 1:/# !initiE 1:/# //= !initiE 1:/# //= /#.
+    + rewrite /get8 /init8. rewrite -H16 1:/# !initiE 1:/# //=.
+    + move => i b *. rewrite H10 1:/#.
+    + rewrite !initiE 1,2:/# get8_set64_directE 1,2:/#.
+    + case(8 * i{!hr} <= i && i < 8 * i{!hr} + 8) => *.
+    + rewrite get64E /init8 pack8bE 1:/# !initiE 1:/# //= !initiE 1:/# //= /#.
+    + rewrite /get8 /init8. rewrite -H17 1:/# !initiE 1:/# //=. smt().
+
+    wp. auto => />. move => &1 &2 H H0 H1 H2 H3 H4 H5 H6 H7 H8 H9 H10 H11 H12 H13 H14 H15 H16.
+    do split;1..6:smt().
+    move => H17 H18. do split. move => *. smt(). move => *. do split. rewrite tP => i ib.
+    rewrite initiE 1:/#. smt(). rewrite tP => i ib. rewrite initiE 1:/#. smt(). rewrite tP => i ib.
+    rewrite initiE 1:/#. smt(). rewrite tP => i ib. rewrite initiE 1:/#. smt().
+
+    wp. auto => />.
+    + seq 3 0 : (#pre /\ ct_X{2} = Array32.init(fun i => ctp{1}.[i+1088])
+                      /\ ct_x25519{1} = Array32.init(fun i => ctp{1}.[i+1088])).
+
+    + while{1} (#pre /\ aux{1} = 4
+                     /\ 0 <= i{1} <= 4
+                     /\ (forall k, 0<=k<min (8 * i{1}) 32 => ctp{1}.[k+1088] = ct_x25519{1}.[k]))
+              (4 - i{1}).
+    + auto => />. move => &hr Z. rewrite !tP.
+    + move => H H0 H1 H2 H3 H4 H5 H6 H7 H8 H9 H10 H11 H12.
+    + move => H13 H14 H15 H16 H17 H18 H19 H20 H21 H22 H23.
+    do split.
+    + move => i b *. rewrite H16 1:/# !initiE 1..3:/#.
+    + rewrite get8_set64_directE 1,2:/# ifF 1:/#.
+    + rewrite /get8 /init8 !initiE 1,2:/# /=.
+    + move => i b *. rewrite H17 1:/# !initiE 1,2:/# //= !initiE 1:/#.
+    + rewrite get8_set64_directE 1,2:/# ifF 1:/#.
+    + rewrite /get8 /init8 !initiE 1,2:/#.
+    + move => i b *. rewrite H18 1:/# !initiE 1..3:/# //=.
+    + rewrite get8_set64_directE 1,2:/# ifF 1:/#.
+    + rewrite /get8 /init8 !initiE 1,2:/#.
+    + move => i b *. rewrite H19 1:/# !initiE 1..2:/# //= !initiE 1:/#.
+    + rewrite get8_set64_directE 1,2:/# ifF 1:/#.
+    + rewrite /get8 /init8 !initiE 1,2:/#.
+    + smt(). smt().
+    + move => i b *. rewrite !initiE 1:/# //=.
+    + rewrite get8_set64_directE 1,2:/#.
+    + case (8 * (136 + i{!hr}) <= i + 1088 && i + 1088 < 8 * (136 + i{!hr}) + 8) => *.
+    + rewrite get64E /init8 pack8bE 1:/# !initiE 1:/# //= !initiE 1:/# //= /#.
+    + rewrite /get8 /init8. rewrite -H22 1:/# !initiE 1,2:/# //= /#. smt().
+
+    wp. simplify. skip => />.
+    move => &1 &2 [#] H H0 H1 H2 H3 H4 H5 H6 H7 H8 H9 H10 H11 H12 H13 H14 H15 H16 H17 H18 H19 H20.
+    do split. smt(). move => [#] H21 H22. do split. move => [#] H23 H24 H25 H26 H27 H28 H29 H30.
+    smt(). move => [#] H31 H32 H33 H34 H35 H36 H37 H38. do split. rewrite tP => i ib.
+    rewrite !initiE 1:/# //=. smt(). rewrite tP => i ib. rewrite !initiE 1:/# //=. smt().
+
+    wp. auto => />.
+    + seq 3 0 : (#pre  /\ ss{2} = shkp{1} /\ ={ss} /\ shkp{1} = ss{1}).
+
+    + while{1} (#pre /\ aux{1} = 4
+                     /\ 0 <= i{1} <= 4
+                     /\ ={ss}
+                     /\ (forall k, 0<=k<min (8 * i{1}) 32 => shkp{1}.[k] = ss{1}.[k])
+                     /\ (forall k, 0<=k<min (8 * i{1}) 32 => shkp{1}.[k] = ss{2}.[k])) (4 - i{1}).
+    + auto => />. move => &hr Z. rewrite !tP.
+    + move => [#] H H0 H1 H2 H3 H4 H5 H6 H7 H8 H9 H10 H11 H12 H13 H14 H15 H16 H17.
+    + move => [#] H18 H19 H20 H21 H22 H23 H24.
+    + do split. smt(). smt().
+    + move => i ib *.  rewrite !initiE 1:/#.
+    + rewrite get8_set64_directE 1,2:/#. case(8 * i{!hr} <= i && i < 8 * i{!hr} + 8) => *.
+    + rewrite get64E /init8 pack8bE 1:/# !initiE 1:/# //= !initiE 1:/# //= /#.
+    + rewrite /get8 /init8 -H23 1:/#. smt(WArray32.initiE).
+    + move => i ib *.  rewrite !initiE 1:/#.
+    + rewrite get8_set64_directE 1,2:/#. case(8 * i{!hr} <= i && i < 8 * i{!hr} + 8) => *.
+    + rewrite get64E /init8 pack8bE 1:/# !initiE 1:/# //= !initiE 1:/# //= /#.
+    + rewrite /get8 /init8 -H23 1:/#. smt(WArray32.initiE).  smt().
+    wp. simplify. skip => />.
+    move => &1 &2 [#] H H0 H1 H2 H3 H4 H5 H6 H7 H8 H9 H10 H11 H12 H13 H14 H15 H16 H17 H18 H19 H20 H21.
+    do split. smt(). move => [#] H22 H23 H24. smt(). move => [#] H24 H25. do split. smt().
+    move => [#] H28 H29 H30 H31. do split. rewrite tP => i ib. smt(). rewrite tP => i ib. smt().
+    auto => />.
 qed.
